\documentclass[11pt]{penrose}

\input{header}

\title{Past Paper: Partial Differential Equations}
\subtitle{OHT-I, 2022}
\begin{document}

\maketitle
\warningtext

\begin{problem}{1}
    % Reduce each of the following equations into canonical form and then find the general solution
    % \begin{enumerate}
    %     \item[(a)] $u_x + 2xy u_y = x$.
    %     \item[(b)] $u_x - y u_y - u = 1$.
    % \end{enumerate}
    
    % \solution\par
    \begin{enumerate}
        \item[(a)] The characteristic equations are
        \begin{equation*}
            \frac{dx}{1} = \frac{dy}{2xy} = \frac{d\xi}{0}.
        \end{equation*}
        So, $\xi = c_1$ and $2x dx = dy/y \implies x^2 = \ln y + c_2$. Here, $c_1$ and $c_2$ are constants. From this, we obtain $\xi = x^2 - \ln y$. Let $\eta = y$. Then
        \begin{equation*}
            u_x = u_\xi \xi_x + u_\eta \eta_x = 2x u_\xi
            \quad\text{and}\quad
            u_y = u_\xi \xi_y + u_\eta \eta_y = -\frac{1}{y} u_\xi + u_\eta.
        \end{equation*}
        Thus, $u_x + 2xy u_y = x$ becomes
        \begin{equation*}
            2x u_\xi -\frac{2xy}{y} u_\xi + 2xy u_\eta = x
            \implies
            2xy u_\eta = x
            \implies
            u_\eta = \frac{1}{y}.
        \end{equation*}
        Therefore, the canonical form is $u_\eta = \frac{1}{\eta}$.

        Integrating by $\eta$, gives $u(\xi, \eta) = f(\xi) + \ln\eta$, where $f$ is an arbitrary function. Consequently,
        \begin{equation*}
            u(x,y) = f(x^2 - \ln y) + \ln y.
        \end{equation*}

        \item[(b)] The characteristic equations are
        \begin{equation*}
            \frac{dx}{1} = \frac{dy}{-y} = \frac{d\xi}{0}.
        \end{equation*}
        So, $\xi = c_1$ and $dx = -dy/y \implies x = -\ln y + c_2$. Here, $c_1$ and $c_2$ are constants. From this, we obtain $\xi = x + \ln y$. Let $\eta = y$. Then
        \begin{equation*}
            u_x = u_\xi \xi_x + u_\eta \eta_x = u_\xi
            \quad\text{and}\quad
            u_y = u_\xi \xi_y + u_\eta \eta_y = \frac{1}{y} u_\xi + u_\eta.
        \end{equation*}
        Thus, $u_x - y u_y - u = 1$ becomes
        \begin{equation*}
            u_\xi - \frac{y}{y} u_\xi - y u_\eta - u = 1
            \implies
            - y u_\eta - u = 1
            \implies
            u_\eta + \frac{1}{y}u = \frac{1}{y}.
        \end{equation*}
        Therefore, the canonical form is $u_\eta + \frac{1}{\eta}u = \frac{1}{\eta}$.

        We solve this as a linear first order ODE. The integrating factor is $e^{\int \frac{1}{\eta} \,d\eta} = \eta$. So,
        \begin{equation*}
            u_\eta + \frac{1}{\eta}u = \frac{1}{\eta}
            \implies
            \eta u_\eta = f(\xi) + \int \frac{\eta}{\eta} \,d\eta
            \implies
            \eta u_\eta = f(\xi) + \eta
            \implies
            u_\eta = \frac{1}{\eta}f(\xi) + 1.
        \end{equation*}
        Therefore, $u(x,y) = \frac{1}{y} \paren*{x + \ln y}$.
    \end{enumerate}
\end{problem}

\begin{problem}{2}
    % Solve the following first-order quasi-linear equation
    % \begin{equation*}
    %     (cy-bz) z_x + (az-cx) z_y = bx-ay
    % \end{equation*}
    
    % \solution
    The characteristic equations are
    \begin{equation*}
        \frac{dx}{cy-bz} = \frac{dy}{az-cx} = \frac{dz}{bx-ay}. \tag*{(\textasteriskcentered)}
    \end{equation*}

    Firstly,
    \begin{equation*}
        \text{(\textasteriskcentered)} = \frac{xdx}{cxy - bxz} = \frac{ydy}{ayz-cxy} = \frac{zdz}{bxz-ayz} = \frac{xdx+ydy+zdz}{0}.
    \end{equation*}
    Therefore, $xdx+ydy+zdz = 0$, and we get $x^2 + y^2 + z^2 = c_1$, where $c_1$ is a constant.

    Next,
    \begin{equation*}
        \text{(\textasteriskcentered)} = \frac{dx}{x(cy-bz)} = \frac{dy}{y(az-cx)} = \frac{adx+bdy}{(ay-bx)c}.
    \end{equation*}
    And,
    \begin{equation*}
        \frac{adx+bdy}{(ay-bx)c} = \frac{dz}{bx-ay}
        \implies \frac{adx+bdy}{c} = -dz
        \implies adx + bdy + cdz = 0
    \end{equation*}
    Therefore, $dx+dy+dz = 0$, and we get $x + y + z = c_2$, where $c_2$ is a constant.

    Thus, the solution is $f(x + y + z, x^2 + y^2 + z^2) = 0$, where $f$ is an arbitrary function.
\end{problem}

\begin{problem}{3}
    % Reduce the following equation into canonical form
    % \begin{equation*}
    %     u_{xx} - u_{yy} + 3u_{x} - 2u_{y} + u = 0.
    % \end{equation*}
    
    % \solution
    Here, $A = 1$, $B = 0$, $C = -1$, $D = 3$ and $E = -2$. So $B^2 - 4AC = 4 > 0$. This is a hyperbolic PDE. The characteristic equation for this PDE is
    \begin{equation*}
        \frac{dy}{dx} = \frac{B \pm \sqrt{B^2 - 4AC}}{2A} = \frac{\pm \sqrt{4}}{2} = \pm 1.
    \end{equation*}
    Upon integration we obtain $y = - x + c_1$ and $y = x + c_2$, where $c_1$ and $c_2$ are constants. Consequently, we have $\xi = y + x$ and $\eta = y - x$. Consequently,
    \begin{align*}
        B^{*} &= 2A\xi_x \eta_x + B \paren*{\xi_x \eta_y + \xi_y \eta_x} + 2C \xi_y \eta_y = -2 + 0 - 2 = -4\\
        D^{*} &= A \xi_{xx} + B \xi_{xy} + C \xi_{yy} + D \xi_{x} + E \xi_{y} = 3-2 = 1,\\
        E^{*} &= A \eta_{xx} + B \eta_{xy} + C \eta_{yy} + D \eta_{x} + E \eta_{y} = -3-2 = -5.
    \end{align*}
    (Note: $A^* = C^* = 0$ because this is a hyperbolic PDE.)

    Thus, the given PDE transforms into $-4 u_{\xi\eta} + u_{\xi} -5 u_{\eta} + u = 0$. This can be re-written as
    \begin{equation*}
        u_{\xi\eta} = \frac{1}{4} u_{\xi} - \frac{5}{4} u_{\eta} + \frac{1}{4} u.
    \end{equation*}
\end{problem}

\begin{problem}{4}
    % Verify that the function
    % \begin{equation*}
    %     u = \varphi(xy) + x \psi\paren*{\frac{y}{x}}
    % \end{equation*}
    % is the general solution of the equation
    % \begin{equation*}
    %     x^2 u_{xx} - y^2 u_{yy} = 0.
    % \end{equation*}

    % \solution
    We have
    \begin{align*}
        u_{x} &= y \varphi'(xy) + \psi\paren*{\frac{y}{x}} - x \paren*{\frac{y}{x^2}} \psi'\paren*{\frac{y}{x}} = y \varphi'(xy) + \psi\paren*{\frac{y}{x}} - \frac{y}{x} \psi'\paren*{\frac{y}{x}}\\
        u_{y} &= x \varphi'(xy) + x \paren*{\frac{1}{x}} \psi'\paren*{\frac{y}{x}} = x \varphi'(xy) + \psi'\paren*{\frac{y}{x}}\\
        u_{xx} &= y^2 \varphi''(xy) - \frac{y}{x^2} \psi'\paren*{\frac{y}{x}} + \frac{y}{x^2} \psi'\paren*{\frac{y}{x}} + \frac{y^2}{x^3} \psi''\paren*{\frac{y}{x}}
        = y^2 \varphi''(xy) + \frac{y^2}{x^3} \psi''\paren*{\frac{y}{x}}\\
        u_{yy} &= x^2 \varphi''(xy) + \frac{1}{x} \psi''\paren*{\frac{y}{x}}
    \end{align*}
    Therefore,
    \begin{equation*}
        x^2 u_{xx} - y^2 u_{yy} = x^2 y^2 \varphi''(xy) + \frac{y^2}{x} \psi''\paren*{\frac{y}{x}} - x^2 y^2 \varphi''(xy) + \frac{y^2}{x} \psi''\paren*{\frac{y}{x}} = 0
    \end{equation*}
\end{problem}

\end{document}